[WIP] int_to_nat opaque op

src/OpaqueOps.v
@@ -65,13 +65,16 @@ Inductive opaque_oper_name : Set :=
 | ONunop (op : int_unop_name)
 | ONbinop (op : int_binop_name)
 | ONtest
-| ONrepr (z : Z).
+| ONrepr (z : Z)
+| ONint_to_nat
+.
 
 Inductive opaque_oper : list type -> type -> Set :=
 | Ounop (op : int_unop_name) : opaque_oper [Opaque Oint] (Opaque Oint)
 | Obinop (op : int_binop_name) : opaque_oper [Opaque Oint; Opaque Oint] (Opaque Oint)
 | Otest : opaque_oper [Opaque Oint] (ADT Tbool)
 | Orepr (z : Z) : opaque_oper [] (Opaque Oint)
+| Oint_to_nat : opaque_oper [Opaque Oint] (ADT Tnat)
 .
 
 Definition opaque_oper_to_name {atys rty} (op : opaque_oper atys rty) : opaque_oper_name :=
@@ -80,6 +83,7 @@ Definition opaque_oper_to_name {atys rty} (op : opaque_oper atys rty) : opaque_o
     | Obinop op => ONbinop op
     | Otest => ONtest
     | Orepr z => ONrepr z
+    | Oint_to_nat => ONint_to_nat
     end.
 
 Definition opaque_oper_name_eq_dec (x y : opaque_oper_name) : { x = y } + { x <> y }.
@@ -87,164 +91,12 @@ decide equality; eauto using Z.eq_dec, int_unop_name_eq_dec, int_binop_name_eq_d
 Defined.
 
 
+Definition num_scratch_vars := 8.
 
-Section MEM_SIM.
-Local Open Scope positive_scope.
-
-Definition closure_sig_higher v :=
-    match v with
-    | HigherValue.Close fname free => Some (fname, length free)
-    | _ => None
-    end.
-
-Definition Plt_dec : forall a b, ({ a < b } + { a >= b })%positive.
-intros. destruct (a ?= b)%positive eqn:?.
-- right. rewrite Pos.compare_eq_iff in *. lia.
-- left. rewrite Pos.compare_lt_iff in *. lia.
-- right. rewrite Pos.compare_gt_iff in *. lia.
-Defined.
-
-Definition pos_range_dec : forall min max x,
-    ({ x >= min /\ x < max } + { x < min \/ x >= max })%positive.
-intros.
-destruct (Plt_dec x min), (Plt_dec x max).
-- right. left. auto.
-- right. left. auto.
-- left. split; auto.
-- right. right. auto.
-Defined.
-
-
-
-Definition mem_sim (mi mi' : block -> option (block * Z)) m1 m1' m2 m2' :=
-    (* mi' maps new blocks on the left to new blocks on the right. *)
-    (forall b,
-        b >= Mem.nextblock m1 ->
-        b < Mem.nextblock m1' ->
-        exists b',
-            mi' b = Some (b', 0%Z) /\
-            b' >= Mem.nextblock m2 /\
-            b' < Mem.nextblock m2') /\
-    (* mi' behaves like mi on old blocks on the left. *)
-    (forall b,
-        b < Mem.nextblock m1 \/ b >= Mem.nextblock m1' ->
-        mi' b = mi b) /\
-    (* The new mappings introduced by mi' are injective. *)
-    (forall b1 b2 b' delta1 delta2,
-        b1 >= Mem.nextblock m1 ->
-        b1 < Mem.nextblock m1' ->
-        b2 >= Mem.nextblock m1 ->
-        b2 < Mem.nextblock m1' ->
-        mi' b1 = Some (b', delta1) ->
-        mi' b2 = Some (b', delta2) ->
-        b1 = b2) /\
-    Mem.nextblock m1 <= Mem.nextblock m1' /\
-    Mem.nextblock m2 <= Mem.nextblock m2'.
-
-Lemma mem_sim_refl : forall mi m1 m1' m2 m2',
-    Mem.nextblock m1 = Mem.nextblock m1' ->
-    Mem.nextblock m2 = Mem.nextblock m2' ->
-    mem_sim mi mi m1 m1' m2 m2'.
-intros0 Hnext1 Hnext2. repeat apply conj; intros.
-- exfalso. rewrite <- Hnext1 in *. lia.
-- reflexivity.
-- exfalso. rewrite <- Hnext1 in *. lia.
-- rewrite Hnext1. lia.
-- rewrite Hnext2. lia.
-Qed.
-
-(* Compose memory simulation "vertically", by adding more steps. *)
-Lemma mem_sim_compose : forall mi mi' mi'' m1 m1' m1'' m2 m2' m2'',
-    mem_sim mi mi' m1 m1' m2 m2' ->
-    mem_sim mi' mi'' m1' m1'' m2' m2'' ->
-    mem_sim mi mi'' m1 m1'' m2 m2''.
-unfold mem_sim. intros0 Hsim Hsim'.
-destruct Hsim as (Hnew & Hold & Hinj & Hext1 & Hext2).
-destruct Hsim' as (Hnew' & Hold' & Hinj' & Hext1' & Hext2').
-repeat apply conj; intros.
-
-- assert (HH : b >= Mem.nextblock m1' \/ b < Mem.nextblock m1'). { lia. } destruct HH.
-  + destruct (Hnew' ?? ** ** ) as (b' & ? & ? & ?).
-    exists b'. repeat apply conj; eauto. lia.
-  + destruct (Hnew ?? ** ** ) as (b' & ? & ? & ?).
-    fwd eapply Hold' as HH; eauto.
-    exists b'. repeat apply conj; eauto.
-    * congruence.
-    * lia.
-
-- eapply eq_trans.
-  + eapply Hold'. break_or; [left; lia | right; eauto].
-  + eapply Hold. break_or; [left; eauto | right; lia].
-
-- destruct (Plt_dec b1 (Mem.nextblock m1')), (Plt_dec b2 (Mem.nextblock m1')).
-
-  + rewrite Hold' in *; eauto.
-
-  + exfalso.
-    (* impossible.  b1 is old, b2 is new, so they can't both map to b'. *)
-    rewrite (Hold' b1) in *; eauto.
-    fwd eapply (Hnew b1) as HH; eauto. destruct HH as (b1' & ? & ? & ?).
-    fwd eapply (Hnew' b2) as HH; eauto. destruct HH as (b2' & ? & ? & ?).
-    assert (b1' = b2') by congruence.
-    assert (b1' < b2') by lia.
-    subst b1'. lia.
-
-  + exfalso.
-    (* impossible.  b1 is old, b2 is new, so they can't both map to b'. *)
-    rewrite (Hold' b2) in *; eauto.
-    fwd eapply (Hnew' b1) as HH; eauto. destruct HH as (b1' & ? & ? & ?).
-    fwd eapply (Hnew b2) as HH; eauto. destruct HH as (b2' & ? & ? & ?).
-    assert (b1' = b2') by congruence.
-    assert (b1' > b2') by lia.
-    subst b1'. lia.
-
-  + eauto.
-
-- lia.
-- lia.
-Qed.
-
-Lemma alloc_mem_sim : forall m1 m2 lo hi m1' b1 mi,
-    Mem.alloc m1 lo hi = (m1', b1) ->
-    Mem.inject mi m1 m2 ->
-    exists mi' m2' b2,
-        Mem.alloc m2 lo hi = (m2', b2) /\
-        Mem.inject mi' m1' m2' /\
-        mem_sim mi mi' m1 m1' m2 m2' /\
-        mi' b1 = Some (b2, 0%Z).
-intros0 Halloc Hinj.
-fwd eapply Mem.alloc_parallel_inject with (lo2 := lo) (hi2 := hi) as HH; eauto.
-  { lia. } { lia. }
-  destruct HH as (mi' & m2' & b2 & ? & ? & ? & ? & ?).
-
-fwd eapply Mem.nextblock_alloc with (m1 := m1); eauto.
-fwd eapply Mem.alloc_result with (m1 := m1); eauto.
-fwd eapply Mem.nextblock_alloc with (m1 := m2); eauto.
-fwd eapply Mem.alloc_result with (m1 := m2); eauto.
-rewrite <- Pos.add_1_l in *.
-
-exists mi', m2', b2. repeat apply conj; eauto.
-unfold mem_sim. repeat apply conj; eauto.
-
-- intros.
-  assert (b = b1). { subst b1. lia. }
-  subst b.
-  exists b2. split; eauto. subst. split; lia.
-
-- intros.
-  assert (b <> b1). { subst b1. lia. }
-  eauto.
-
-- intros b1' b2'. intros.
-  assert (b1' = Mem.nextblock m1) by (zify; lia).
-  assert (b2' = Mem.nextblock m1) by (zify; lia).
-  congruence.
-
-- lia.
-- lia.
-Qed.
-
-End MEM_SIM.
+Record cminor_codegen_context := CminorCodegenContext {
+    cmcc_malloc_id : ident;
+    cmcc_scratch : list ident
+}.
 
 Record opaque_oper_impl {atys rty} := MkOpaqueOperImpl {
         oo_denote : hlist type_denote atys -> type_denote rty;
@@ -253,7 +105,7 @@ Record opaque_oper_impl {atys rty} := MkOpaqueOperImpl {
         oo_denote_higher : list HigherValue.value -> option HigherValue.value;
         oo_denote_high : list HighValues.value -> option HighValues.value;
         oo_denote_mem_effect : mem -> list val -> option (mem * val);
-        oo_denote_cminor : ident -> ident -> list Cminor.expr -> Cminor.stmt;
+        oo_denote_cminor : cminor_codegen_context -> ident -> list Cminor.expr -> Cminor.stmt;
 
         (* properties *)
         (* "No fabricated closures."  Every closure in the output must be
@@ -313,14 +165,16 @@ Record opaque_oper_impl {atys rty} := MkOpaqueOperImpl {
             exists m' ret',
                 oo_denote_mem_effect m args' = Some (m', ret') /\
                 HighValues.value_inject ge m' ret ret';
-        oo_sim_cminor : forall (ge : genv) f malloc_id id e m m' sp k fp,
+        oo_sim_cminor : forall (ge : genv) f ctx id e m m' sp k fp,
             forall args argvs retv,
             oo_denote_mem_effect m argvs = Some (m', retv) ->
             eval_exprlist ge sp e m args argvs ->
-            Genv.find_symbol ge malloc_id = Some fp ->
+            Genv.find_symbol ge (cmcc_malloc_id ctx) = Some fp ->
             Genv.find_funct ge (Vptr fp Int.zero) = Some (External EF_malloc) ->
-            (* TODO: need a premise that the `args` exprs don't touch `e ! id` *)
-            plus Cminor.step ge (State f (oo_denote_cminor malloc_id id args) k sp e m)
+            length (cmcc_scratch ctx) >= num_scratch_vars ->
+            Forall (fun id' => Forall (expr_no_access id') args) (cmcc_scratch ctx) ->
+            Forall (expr_no_access id) args ->
+            plus Cminor.step ge (State f (oo_denote_cminor ctx id args) k sp e m)
                              E0 (State f Sskip k sp (PTree.set id retv e) m')
     }.
 
@@ -456,7 +310,7 @@ simple refine (MkOpaqueOperImpl _ _  _ _ _ _ _ _ _  _ _ _ _  _ _ _ _ _ _).
     | [Vint x] => Some (m, Vint (int_unop_denote op x))
     | _ => None
     end).
-- refine (fun _malloc_id id args =>
+- refine (fun _ctx id args =>
     match args with
     | [x] => Sassign id (int_unop_to_cminor op x)
     | _ => Sskip
@@ -604,7 +458,7 @@ simple refine (MkOpaqueOperImpl _ _  _ _ _ _ _ _ _  _ _ _ _  _ _ _ _ _ _).
     | [Vint x; Vint y] => Some (m, Vint (int_binop_denote op x y))
     | _ => None
     end).
-- refine (fun _malloc_id id args =>
+- refine (fun _ctx id args =>
     match args with
     | [x; y] => Sassign id (int_binop_to_cminor op x y)
     | _ => Sskip
@@ -738,18 +592,15 @@ simple refine (MkOpaqueOperImpl _ _  _ _ _ _ _ _ _  _ _ _ _  _ _ _ _ _ _).
     match args with
     | [Vint x] =>
             let tag := if Int.eq x Int.zero then Int.zero else Int.one in
-            match build_constr m tag [] with
-            | Some (ret, m') => Some (m', ret)
-            | None => None
-            end
+            build_constr m tag []
     | _ => None
     end).
-- refine (fun malloc_id id args =>
+- refine (fun ctx id args =>
     match args with
     | [e] =>
             Sifthenelse (Ebinop (Ocmpu Ceq) e (Econst (Ointconst Int.zero)))
-                (build_constr_cminor malloc_id id Int.zero [])
-                (build_constr_cminor malloc_id id Int.one [])
+                (build_constr_cminor (cmcc_malloc_id ctx) id Int.zero [])
+                (build_constr_cminor (cmcc_malloc_id ctx) id Int.one [])
     | _ => Sskip
     end).
 
@@ -778,29 +629,11 @@ simple refine (MkOpaqueOperImpl _ _  _ _ _ _ _ _ _  _ _ _ _  _ _ _ _ _ _).
   rename m2 into m3, m0 into m2, m1 into m0, m into m1.
   rename m1' into m0'.
 
-  (* TODO: pull this out as a lemma about build_constr *)
-
-  fwd eapply alloc_mem_sim as HH; eauto.
-    destruct HH as (mi' & m1' & b' & ? & ? & ? & ?).
-
-  fwd eapply Mem.store_mapped_inject with (m1 := m1) as HH; eauto.
-    destruct HH as (m2' & ? & ?).
-
-  fwd eapply Mem.store_mapped_inject with (m1 := m2) as HH; eauto.
-    destruct HH as (m3' & ? & ?).
-
-  eexists mi', m3', _.
-  split; cycle 1.
-    { split; [|split]; eauto.
-      eapply mem_sim_compose; cycle 1.
-        { eapply mem_sim_refl; symmetry; eapply Mem.nextblock_store; eauto. }
-      eapply mem_sim_compose; cycle 1.
-        { eapply mem_sim_refl; symmetry; eapply Mem.nextblock_store; eauto. }
-      eauto. }
-
+  eapply build_constr_mem_inject; eauto.
   unfold build_constr.
-  simpl in *.
-  repeat (on _, fun H => rewrite H; simpl).
+  find_rewrite. eapply require_bind_eq. { constructor. } intro.
+  simpl. find_rewrite. simpl.
+  find_rewrite. simpl.
   reflexivity.
 
 
@@ -850,10 +683,9 @@ simple refine (MkOpaqueOperImpl _ _  _ _ _ _ _ _ _  _ _ _ _  _ _ _ _ _ _).
     { rewrite Zcomplements.Zlength_nil. eapply max_arg_count_big. lia. }
     destruct HH as (ret' & m' & ? & ?).
   exists m', ret'. split; eauto.
-  find_rewrite. reflexivity.
 
 - intros. simpl in *.
-  do 5 (break_match_hyp; try discriminate).  on (_ * _)%type, fun H => destruct H.
+  do 4 (break_match_hyp; try discriminate).
   do 2 on >eval_exprlist, invc.
   inject_some.
 
@@ -868,7 +700,7 @@ simple refine (MkOpaqueOperImpl _ _  _ _ _ _ _ _ _  _ _ _ _  _ _ _ _ _ _).
   }
 
   replace (if Int.eq i _ then _ else _) with
-      (build_constr_cminor malloc_id id
+      (build_constr_cminor (cmcc_malloc_id ctx) id
         (if Int.eq i Int.zero then Int.zero else Int.one) []); cycle 1.
     { destruct (Int.eq _ _); reflexivity. }
 
@@ -892,7 +724,7 @@ simple refine (MkOpaqueOperImpl _ _  _ _ _ _ _ _ _  _ _ _ _  _ _ _ _ _ _).
 - refine (fun args => Some (HigherValue.Opaque Oint (Int.repr z))).
 - refine (fun args => Some (HighValues.Opaque Oint (Int.repr z))).
 - refine (fun m args => Some (m, Vint (Int.repr z))).
-- refine (fun _malloc_id id args => Sassign id (Econst (Ointconst (Int.repr z)))).
+- refine (fun _ctx id args => Sassign id (Econst (Ointconst (Int.repr z)))).
 
 
 - (* no_fab_clos_higher *)
@@ -922,6 +754,397 @@ simple refine (MkOpaqueOperImpl _ _  _ _ _ _ _ _ _  _ _ _ _  _ _ _ _ _ _).
 Defined.
 
 
+Lemma Acc_func' : forall A (RA : A -> A -> Prop) B (RB : B -> B -> Prop) (f : A -> B) (b : B),
+    (forall a1 a2, RA a1 a2 -> RB (f a1) (f a2)) ->
+    Acc RB b ->
+    forall (a : A), f a = b ->
+    Acc RA a.
+intros0 Hrel. induction 1. intros0 Heq. constructor.
+intros a' ?. eapply H0. rewrite <- Heq. eapply Hrel.
+eassumption.
+reflexivity.
+Qed.
+
+Lemma Acc_func : forall A (RA : A -> A -> Prop) B (RB : B -> B -> Prop) (f : A -> B) (a : A),
+    (forall a1 a2, RA a1 a2 -> RB (f a1) (f a2)) ->
+    Acc RB (f a) ->
+    Acc RA a.
+intros. eapply Acc_func'; eauto.
+Qed.
+
+Lemma int_ltu_well_founded : well_founded (fun a b => Int.ltu a b = true).
+unfold well_founded. intros i.
+eapply Acc_func with (f := Int.unsigned) (RB := fun a b => (0 <= a < b)%Z).
+  { intros. eapply Int.ltu_inv; eauto. }
+eapply (Z.lt_wf 0).
+Qed.
+
+Lemma int_nonzero_pred : forall i,
+    Int.eq i Int.zero = false ->
+    Int.unsigned (Int.sub i Int.one) = (Int.unsigned i - 1)%Z.
+intros.
+
+assert (0 < Int.unsigned i < Int.modulus)%Z.
+  { fwd eapply Int.unsigned_range with (i := i); eauto.
+    unfold Int.eq in *. break_if; try discriminate. rewrite Int.unsigned_zero in *.
+    lia. }
+
+unfold Int.sub in *. rewrite Int.unsigned_one in *.
+rewrite Int.unsigned_repr in *; cycle 1.
+  {  unfold Int.max_unsigned. lia. }
+lia.
+Qed.
+
+Function int_iter {A} (f : A -> A) (n : int) (x : A)
+        {measure (fun n => Z.to_nat (Int.unsigned n)) n} : A :=
+    if Int.eq n Int.zero then x else f (int_iter f (Int.sub n Int.one) x).
+Proof.
+intros.
+
+eapply Z2Nat.inj_lt.
+  { fwd eapply Int.unsigned_range. break_and. eassumption. }
+  { fwd eapply Int.unsigned_range. break_and. eassumption. }
+
+rewrite int_nonzero_pred by eauto. lia.
+Qed.
+Arguments int_iter [A] f n x : rename.
+
+Check nat_rect.
+
+Lemma int_peano_rect (P : int -> Type)
+    (H0 : P Int.zero) 
+    (HS : forall i, i <> Int.zero -> P (Int.sub i Int.one) -> P i)
+    : forall i, P i.
+eapply (well_founded_induction_type int_ltu_well_founded).
+intros i IHi.
+
+destruct (Int.eq i Int.zero) eqn:?.
+  { fwd eapply Int.eq_ok as HH; eauto. subst i. exact H0. }
+
+eapply HS.
+- contradict Heqb. subst. rewrite Int.eq_true. discriminate.
+- eapply IHi.
+  unfold Int.ltu. rewrite int_nonzero_pred; eauto.
+  break_if; try reflexivity. lia.
+Qed.
+
+Lemma int_to_nat_iter : forall i,
+    Z.to_nat (Int.unsigned i) = int_iter S i O.
+induction i using int_peano_rect; rewrite int_iter_equation.
+  { rewrite Int.eq_true. reflexivity. }
+
+rewrite Int.eq_false by eauto.
+
+replace (Int.unsigned i) with ((1 + Int.unsigned (Int.sub i (Int.one)))%Z); cycle 1.
+  { rewrite int_nonzero_pred; cycle 1.
+      { on (i <> Int.zero), eapply_lem Int.eq_false. eauto. }
+    lia. }
+
+rewrite Z2Nat.inj_add; cycle 1.
+  { lia. }
+  { fwd eapply Int.unsigned_range. break_and. eauto. }
+simpl.
+
+congruence.
+Qed.
+
+Lemma mem_sim_same_offsets : forall mi mi' m1 m1' m2 m2',
+    same_offsets mi ->
+    mem_sim mi mi' m1 m1' m2 m2' ->
+    same_offsets mi'.
+intros0 Hoff Hsim. unfold same_offsets in *. intros.
+destruct Hsim as (Hnew & Hold & Hinj & Hext1 & Hext2).
+destruct (pos_range_dec (Mem.nextblock m1) (Mem.nextblock m1') b).
+- break_and. fwd eapply Hnew as HH; eauto. destruct HH as (b'' & ? & ? & ?).
+  congruence.
+- rewrite Hold in * by eauto. eauto.
+Qed.
+
+
+
+Lemma store_multi_valid_block : forall chunk m1 b ofs vs m2,
+    store_multi chunk m1 b ofs vs = Some m2 ->
+    forall b', Mem.valid_block m1 b' -> Mem.valid_block m2 b'.
+first_induction vs; intros0 Hstore; intros0 Hb; simpl in *.
+- inject_some. eauto.
+- break_match; try discriminate.
+  eapply Mem.store_valid_block_1 in Hb; cycle 1. { eassumption. }
+  eauto.
+Qed.
+
+Lemma build_constr_valid_ptr : forall m1 tag args m2 ret,
+    build_constr m1 tag args = Some (m2, ret) ->
+    valid_ptr m2 ret.
+intros0 Hbuild. unfold build_constr in Hbuild.
+break_match. rewrite Z.add_comm in *. break_bind_option. inject_some.
+simpl.
+eapply store_multi_valid_block; eauto.
+eapply Mem.store_valid_block_1; eauto.
+eapply Mem.store_valid_block_1; eauto.
+eapply Mem.valid_new_block; eauto.
+Qed.
+
+Definition impl_int_to_nat : opaque_oper_impl [Opaque Oint] (ADT Tnat).
+simple refine (MkOpaqueOperImpl _ _  _ _ _ _ _ _ _  _ _ _ _  _ _ _ _ _ _).
+
+- exact (fun args => Z.to_nat (Int.unsigned (hhead args))).
+- refine (fun G args =>
+    let x := unwrap_opaque (hhead args) in
+    int_iter (fun n => VConstr CTS (hcons n hnil)) x (VConstr CTO hnil)).
+- refine (fun args =>
+    match args with
+    | [HighestValues.Opaque Oint x] => Some (int_iter
+            (fun n => HighestValues.Constr CS [n])
+            x
+            (HighestValues.Constr CO []))
+    | _ => None
+    end).
+- refine (fun args =>
+    match args with
+    | [HigherValue.Opaque Oint x] => Some (int_iter
+            (fun n => HigherValue.Constr 1 [n])
+            x
+            (HigherValue.Constr 0 []))
+    | _ => None
+    end).
+- refine (fun args =>
+    match args with
+    | [HighValues.Opaque Oint x] => Some (int_iter
+            (fun n => HighValues.Constr Int.one [n])
+            x
+            (HighValues.Constr Int.zero []))
+    | _ => None
+    end).
+- refine (fun m args =>
+    match args with
+    | [Vint x] => int_iter
+            (fun m_v =>
+                match m_v with
+                | Some (m, v) =>
+                        build_constr m Int.one [v]
+                | None => None
+                end)
+            x
+            (build_constr m Int.zero [])
+    | _ => None
+    end).
+- Check nth. refine (fun ctx id args =>
+    let counter := nth 0 (cmcc_scratch ctx) 1%positive in
+    let tmp := nth 1 (cmcc_scratch ctx) 1%positive in
+    match args with
+    | [e] => Sseq (Sseq
+            (Sassign counter e)
+            (build_constr_cminor (cmcc_malloc_id ctx) id Int.zero []))
+            (Sblock (Sloop
+                (Sifthenelse (Ebinop (Ocmpu Ceq) (Evar counter) (Econst (Ointconst Int.zero)))
+                    (Sexit 0)
+                    (Sseq (Sseq
+                        (Sassign tmp (Evar id))
+                        (build_constr_cminor (cmcc_malloc_id ctx) id Int.one [Evar id]))
+                        (Sassign counter (Ebinop
+                            Osub (Evar counter) (Econst (Ointconst Int.one))))
+                    )
+                )
+            ))
+    | _ => Sskip
+    end).
+
+
+- (* no_fab_clos_higher *)
+  intros. simpl in *.
+  repeat (break_match; try discriminate; [ ]). subst. inject_some.
+  cut (closure_sig_higher v = None). { intro. exfalso. congruence. }
+  clear dependent sig.
+  rename v1 into i.  revert i v H0. simpl.
+  induction i using int_peano_rect; rewrite int_iter_equation;
+    rewrite Int.eq_true + rewrite Int.eq_false; intros; eauto.
+  all: on >HigherValue.VIn, invc; eauto.
+  + contradiction.
+  + break_or; [ | contradiction ]. eauto.
+
+- (* change_fname_high *)
+  intros. simpl in *.
+  repeat (break_match_hyp; try discriminate; [ ]).
+  repeat on >Forall2, invc. simpl in *. break_match; try contradiction.
+  fix_existT. subst. inject_some.
+  eexists; split; eauto.
+
+  rename v into i. simpl in i.
+  induction i using int_peano_rect; rewrite int_iter_equation;
+    rewrite Int.eq_true + rewrite Int.eq_false; intros; eauto.
+  + repeat econstructor.
+  + repeat (eassumption || econstructor).
+
+- (* mem_inj_id *)
+  intros. simpl in *. repeat (break_match_hyp; try discriminate; []). subst. inject_some.
+  revert i m m' ret H.
+  induction i using int_peano_rect; intros ? ? ?; rewrite int_iter_equation;
+    rewrite Int.eq_true + rewrite Int.eq_false; intros; eauto.
+  + repeat (break_match; try discriminate). inject_some.
+    eapply build_constr_mem_inj_id; eauto.
+  + repeat ((break_match; []) || (break_match; [ | discriminate ])).
+    subst.  inject_some.
+    rewrite <- inject_id_compose_self. eapply Mem.mem_inj_compose.
+    * eapply IHi; eauto.
+    * eapply build_constr_mem_inj_id; eauto.
+
+- (* mem_inject *)
+  intros. simpl in *. repeat (break_match_hyp; try discriminate; []). subst. inject_some.
+  do 2 on >Forall2, invc. on >Val.inject, invc.
+
+  (* this is roughly `eassert` / `ecut` *)
+  fwd instantiate (1 := valid_ptr m2 ret /\
+        exists (mi' : meminj) (m2' : mem) (ret' : val),
+            valid_ptr m2' ret' /\ _ mi' m2' ret' ) as HH.
+    all: cycle 1.
+    { destruct HH as (? & (mi' & m2' & ret' & ? & HH)).
+      exists mi', m2', ret'. pattern mi', m2', ret'. exact HH. }
+  simpl.
+
+  revert i mi m1 m2 m1' ret H H0 H1.
+  induction i using int_peano_rect; intros ? ? ?.
+  all: rewrite int_iter_equation; rewrite Int.eq_true + rewrite Int.eq_false; intros; eauto.
+  all: rewrite int_iter_equation; rewrite Int.eq_true + rewrite Int.eq_false; eauto.
+
+    { split.
+        { eapply build_constr_valid_ptr. eauto. }
+      fwd eapply build_constr_mem_inject as HH; eauto.
+        destruct HH as (mi' & m2' & v2 & ? & ? & ? & ?).
+      eauto 10 using build_constr_valid_ptr. }
+
+  do 2 (break_match_hyp; try discriminate). subst.
+  fwd eapply IHi as HH; eauto.
+    destruct HH as (? & (mi' & m2' & ret' & ? & ? & ? & ? & ?)).
+  find_rewrite.
+  fwd eapply build_constr_mem_inject as HH; eauto.
+    { eapply mem_sim_same_offsets; eauto. }
+    destruct HH as (mi'' & m2'' & v'' & ? & ? & ? & ?).
+  split.
+    { eapply build_constr_valid_ptr; eauto. }
+  exists mi'', m2'', v''.
+  do 4 try eapply conj.
+  + eapply build_constr_valid_ptr; eauto.
+  + eauto.
+  + eauto.
+  + eauto.
+  + eauto using mem_sim_compose.
+
+
+- intros. simpl.
+  rewrite hmap_hhead.  rewrite opaque_value_denote.
+  rewrite int_to_nat_iter.
+  remember (unwrap_opaque (hhead vs)) as i. clear Heqi.
+  induction i using int_peano_rect; rewrite int_iter_equation.
+  all: rewrite int_iter_equation with (x := VConstr CTO hnil).
+  all: rewrite Int.eq_true + rewrite Int.eq_false; intros; eauto.
+  simpl. congruence.
+
+- intros. simpl in *.
+  revert H.
+  on _, invc_using (@case_hlist_cons type). on _, invc_using (@case_hlist_nil type).
+  on _, invc_using case_value_opaque.
+  simpl.
+  rename ov into i. simpl in i.
+  induction i using int_peano_rect; rewrite int_iter_equation.
+  all: rewrite int_iter_equation with (x := VConstr CTO hnil).
+  all: rewrite Int.eq_true + rewrite Int.eq_false; intros; eauto.
+  simpl. congruence.
+
+- intros. simpl in *.
+
+  on >Forall2, invc; try discriminate.
+  on >mv_higher, invc; try discriminate.
+  destruct oty; try discriminate.
+  on >Forall2, invc; try discriminate.
+  inject_some.
+
+  eexists. split; eauto.
+
+  rename ov into i. simpl in i.
+  induction i using int_peano_rect; rewrite int_iter_equation.
+  all: rewrite int_iter_equation with (x := HigherValue.Constr 0 []).
+  all: rewrite Int.eq_true + rewrite Int.eq_false; intros; eauto.
+  + econstructor; eauto.
+  + econstructor; eauto.
+
+- intros. simpl in *.
+
+  on >Forall2, invc; try discriminate.
+  on >mv_high, invc; try discriminate.
+  destruct oty; try discriminate.
+  on >Forall2, invc; try discriminate.
+  inject_some.
+
+  eexists. split; eauto.
+
+  rename ov into i. simpl in i.
+  induction i using int_peano_rect; rewrite int_iter_equation.
+  all: rewrite int_iter_equation with (x := HighValues.Constr Int.zero []).
+  all: rewrite Int.eq_true + rewrite Int.eq_false; intros; eauto.
+  + econstructor; eauto.
+  + econstructor; eauto.
+
+- intros. simpl in *.
+
+  on >Forall2, invc; try discriminate.
+  on >@HighValues.value_inject, invc; try discriminate.
+  destruct oty; try discriminate.
+  on >Forall2, invc; try discriminate.
+  inject_some.
+
+  on >opaque_type_value_inject, invc.
+
+  rename ov into i. simpl in i.
+  induction i using int_peano_rect; rewrite int_iter_equation.
+  all: rewrite int_iter_equation with (x := HighValues.Constr Int.zero []).
+  all: rewrite Int.eq_true + rewrite Int.eq_false; intros; eauto.
+
+  + fwd eapply build_constr_ok as HH; eauto.
+      { rewrite Zlength_nil. eapply max_arg_count_big. lia. }
+      destruct HH as (v & m2 & ? & ?).
+    eauto.
+
+  + destruct IHi as (m' & ret' & ? & ?).
+    find_rewrite.
+    fwd eapply build_constr_ok with (m1 := m') (args := [ret']) as HH.
+      { econstructor; eauto. }
+      { rewrite Zlength_correct. simpl. eapply max_arg_count_big. lia. }
+      destruct HH as (ret'' & m'' & ? & ?).
+    eauto.
+
+- admit. (*intros. simpl in *.
+  do 5 (break_match_hyp; try discriminate).  on (_ * _)%type, fun H => destruct H.
+  do 2 on >eval_exprlist, invc.
+  inject_some.
+
+  eapply plus_left. 3: eapply E0_E0_E0. {
+    econstructor.
+    - econstructor; eauto.
+        { econstructor. simpl. reflexivity. }
+      simpl. unfold Val.cmpu. simpl. reflexivity.
+    - simpl.
+      instantiate (1 := Int.eq i Int.zero).
+      destruct (Int.eq _ _); econstructor.
+  }
+
+  replace (if Int.eq i _ then _ else _) with
+      (build_constr_cminor malloc_id id
+        (if Int.eq i Int.zero then Int.zero else Int.one) []); cycle 1.
+    { destruct (Int.eq _ _); reflexivity. }
+
+  eapply plus_star. eapply build_constr_cminor_effect.
+  + eauto.
+  + econstructor.
+  + econstructor.
+  + rewrite Zlength_correct. simpl. eapply max_arg_count_big. lia.
+  + eauto.
+  + eauto.
+    *)
+
+(*Defined.*)
+Admitted.
+
+
 
 
 
@@ -935,6 +1158,7 @@ Definition get_opaque_oper_impl {atys rty} (op : opaque_oper atys rty) :
     | Obinop op => impl_binop op
     | Otest => impl_test
     | Orepr z => impl_repr z
+    | Oint_to_nat => impl_int_to_nat
     end.
 
 Definition get_opaque_oper_impl' (op : opaque_oper_name) :
@@ -944,6 +1168,7 @@ Definition get_opaque_oper_impl' (op : opaque_oper_name) :
     | ONbinop op => existT _ _ (existT _ _ (impl_binop op))
     | ONtest => existT _ _ (existT _ _ impl_test)
     | ONrepr z => existT _ _ (existT _ _ (impl_repr z))
+    | ONint_to_nat => existT _ _ (existT _ _ (impl_int_to_nat))
     end.
 
 Lemma get_opaque_oper_impl_name : forall atys rty (op : opaque_oper atys rty),
@@ -1082,13 +1307,16 @@ clearbody impl'. destruct impl' as (? & ? & impl'').
 eapply (oo_sim_mem_effect impl''); eauto.
 Qed.
 
-Lemma opaque_oper_sim_cminor : forall (ge : genv) f malloc_id id e m m' sp k fp,
+Lemma opaque_oper_sim_cminor : forall (ge : genv) f ctx id e m m' sp k fp,
     forall args argvs retv,
     opaque_oper_denote_mem_effect m argvs = Some (m', retv) ->
     eval_exprlist ge sp e m args argvs ->
-    Genv.find_symbol ge malloc_id = Some fp ->
+    Genv.find_symbol ge (cmcc_malloc_id ctx) = Some fp ->
     Genv.find_funct ge (Vptr fp Int.zero) = Some (External EF_malloc) ->
-    plus Cminor.step ge (State f (opaque_oper_denote_cminor malloc_id id args) k sp e m)
+    length (cmcc_scratch ctx) >= num_scratch_vars ->
+    Forall (fun id' => Forall (expr_no_access id') args) (cmcc_scratch ctx) ->
+    Forall (expr_no_access id) args ->
+    plus Cminor.step ge (State f (opaque_oper_denote_cminor ctx id args) k sp e m)
                      E0 (State f Sskip k sp (PTree.set id retv e) m').
 intros0 Hmv HH. unfold opaque_oper_denote_mem_effect, opaque_oper_denote_cminor in *.
 clearbody impl'. destruct impl' as (? & ? & impl'').
